{
 "cells": [
  {
   "cell_type": "markdown",
   "metadata": {},
   "source": [
    "#### 1.13 \n",
    "\n",
    "Let $X_1, \\ldots, X_n$ be independent random variables, all having the same distribution with expected values $\\mu$ and variance $\\sigma^2$  The Random Variable $\\bar{X}$, defined as the arithmetic average of these variables is called the sample mean.  That is, the sample mean is given by: \n",
    "\n",
    "$\\bar{X} = \\frac{\\Sigma^n_{i =1}X_i}{n}$\n",
    "\n",
    "(a) Show that $E[\\bar{X}] = \\mu$\n",
    "\n",
    "(b) Show that $Var(\\bar{X}) = \\frac{\\sigma^2}{n}$\n",
    "\n",
    "The random variable $S^2$ is called the sample variance, defined by: \n",
    "\n",
    "$ S^2 = \\frac{\\Sigma^n_{i = 1}(X_i -\\bar{X})^2}{n-1}$\n",
    "\n",
    "(c) Show that $\\Sigma^n_{i = 1}(X_i -\\bar{X})^2 = \\Sigma^n_{i = 1}X_{i}^2 - n\\bar{X}^2$\n",
    "\n",
    "(d) Show that $E[S^2] = \\sigma^2$\n",
    "\n",
    "##### 1.13a Solution\n",
    "\n",
    "$E[\\bar{X}]$\n",
    "\n",
    "$ = E[\\frac{\\Sigma^n_{i =1}X_i}{n}] = \\frac{1}{n}E[\\Sigma^n_{i =1}X_i]$ `by proposition 1.3.1`\n",
    "\n",
    "given that $\\frac{1}{n} (E[X_1] + E[X_2] + \\ldots + E[X_n]) = \\mu$\n",
    "\n",
    "then $\\frac{1}{n} (\\mu_1 + \\mu_2 + \\ldots \\mu_n) = \\mu$\n",
    "\n",
    "##### 1.13b Solution\n",
    "\n",
    "$Var(\\bar{X}) = Var (\\frac{\\Sigma_{i = 1}^n X_i}{n})$\n",
    "\n",
    "$= (\\frac{1}{n}^2 Var(X_1 + X_2 + \\ldots + X_n)$. `from equation 1.8 and expanding the summation`\n",
    "\n",
    "$ = (\\frac{1}{n}^2 (\\sigma_1^2 + \\sigma_2^2 + \\ldots + \\sigma_n^2)$ `given prop 1.3.2 and the stated variance`\n",
    "\n",
    "$ = (\\frac{1}{n})^2 \\cdot n\\sigma^2 $\n",
    "\n",
    "$ = \\frac{\\sigma^2}{n}$\n",
    "\n",
    "\n",
    "##### 1.13c Solution\n",
    "\n",
    "Expand the binomial \n",
    "\n",
    "$\\Sigma_{i =1} ^n (X_i - \\bar{X})^2 = \\Sigma_{i = 1}^n (X_i^2 - 2X \\bar{X} + \\bar{X}^2)$\n",
    "\n",
    "$ = \\Sigma_{i = 1}^n X_i^2  + \\Sigma_{i = 1}^n 2X_i \\bar{X}  +\\Sigma_{i = 1}^n  \\bar{X}^2$\n",
    "\n",
    "using the useful identity\n",
    "\n",
    " $\\Sigma X_i = n\\bar{X}$\n",
    "\n",
    "we substitue in and get\n",
    "\n",
    "$\\Sigma_{i = 1}^n X_i ^2 - 2n \\bar{X}^2 + n \\bar{X}^2$\n",
    "\n",
    "and combine like terms\n",
    "\n",
    "$\\Sigma_{i = 1}^n X_i^2 -n\\bar{X}^2$\n",
    "\n",
    "\n",
    "\n",
    "\n",
    "\n",
    "\n",
    "##### 1.13d Solution\n",
    "\n",
    "L.H.S.  $E[S^2] = E[\\frac{\\Sigma(X_i - \\bar{X})^2}{n-1}]$\n",
    "\n",
    "$(n-1)E(S^2) = E[\\Sigma(X_i - \\bar{X})^2]$\n",
    "\n",
    "\n",
    "Then for R.H.S\n",
    "we expand out... \n",
    "\n",
    "$E[\\Sigma(X_i - 2X_i\\bar{X} + \\bar{X}^2)]$\n",
    "\n",
    "$E[\\Sigma X_i^2 - 2\\bar{X}\\Sigma X_i + \\Sigma \\bar{X}^2]$\n",
    "\n",
    "$E[\\Sigma X_i^2 - 2n\\bar{X} + n\\bar{X}^2]$.   Note that $\\Sigma \\bar{X}^2 = n\\bar{X}^2$ and $\\Sigma X_i = n\\bar{X}$\n",
    "\n",
    "$=E[\\Sigma X_i^2 - n\\bar{X}^2] = \\Sigma E[X_i]^2 - E[n\\bar{X}^2]$ using proposition 1.3.1\n",
    "\n",
    "$= \\Sigma E[X_i]^2 - n E[\\bar{X}^2]$\n",
    "\n",
    "`Special substitution notes`\n",
    "\n",
    "1. $Var(\\bar{X}) = E[\\bar{X}^2] - (E[\\bar{X}])^2$\n",
    "\n",
    "therefore $E[\\bar{X}^2] = \\frac{\\sigma^2}{n} + \\mu^2$\n",
    "\n",
    "2. $Var(X) = E[X^2] - (E[X])^2$\n",
    "\n",
    "therefore $E[X^2] = \\sigma^2 + \\mu^2$\n",
    "\n",
    "Then \n",
    "\n",
    "$ = \\Sigma(\\sigma^2 + \\mu^2) - n(\\frac{\\sigma^2}{n} + \\mu^2)$\n",
    "\n",
    "$= n\\sigma^2 + n\\mu^2  - \\sigma^2 - n\\mu^2$\n",
    "\n",
    "$= (n-1)\\sigma^2$\n",
    "\n",
    "Going back to the top \n",
    "\n",
    "$(n-1)E[S^2] = (n-1)\\sigma^2$\n",
    "\n",
    "therefore $E[S^2] = \\sigma^2$\n",
    "\n",
    "##### 1.13d"
   ]
  },
  {
   "cell_type": "markdown",
   "metadata": {},
   "source": [
    "\n",
    "#### 1.14\n",
    "\n",
    "Verify that $Cov(X,Y) = E[XY] - E[X][Y]$\n",
    "\n",
    "\n",
    "##### 1.14 Solution\n",
    "\n",
    "Given $E[X] = \\mu$\n",
    "\n",
    "$Cov(X,Y) = E[(X - E[X)(Y-E[Y])]$ \n",
    "\n",
    "$ = E[(XY - XE[Y] - E[X]Y + \\mu_X\\mu_Y)]$\n",
    "\n",
    "$ =E[(XY - X\\mu_Y - Y\\mu_X + \\mu_X \\mu_Y)]$\n",
    "\n",
    "$ = E[XY] - \\mu_YE[X] - \\mu_XE[Y] + \\mu_x \\mu_Y$ `by 1.7`\n",
    "\n",
    "$ = E[XY] - E[Y]E[X] - E[X]E[Y] + E[X]E[Y]$\n",
    "\n",
    "$ = E[XY] - E[X][Y]$\n"
   ]
  },
  {
   "cell_type": "markdown",
   "metadata": {},
   "source": [
    "#### 1.15a \n",
    "\n",
    "Prove $Cov(XY) = Cov(YX)$\n",
    "\n",
    "##### 1.15a solution\n",
    "$Cov (X,Y) = E[(X - E[X])(Y - E[Y])]$\n",
    "\n",
    "$ = E[(Y - E[Y])(X-E[X]]$ `by commutative property`\n",
    "\n",
    "$ = Cov(Y,X)$\n",
    "\n",
    "#### 1.15c\n",
    "\n",
    "Prove $Cov(cX,Y) = cCov(X, Y)$ \n",
    "\n",
    "##### 1.15c Solution\n",
    "\n",
    "$Cov(cX,Y) = E[c(X - E[x]) (Y - E[Y])]$\n",
    "\n",
    "$=E[cXY - cX\\mu_Y - cY\\mu_X + c\\mu_X \\mu_Y]$ \n",
    "\n",
    "$=cE[XY] - c\\mu_Y\\mu_X - cY\\mu_X + c\\mu_X\\mu_Y$\n",
    "\n",
    "$=c(E[XY] - E[X]E[Y])$\n",
    "\n",
    "$=cCov(X,Y)$"
   ]
  },
  {
   "cell_type": "markdown",
   "metadata": {},
   "source": [
    "#### 1.16 \n",
    "\n",
    "If U and V are independent random variables, both having variance 1, find $Cov(X,Y)$ when: \n",
    "\n",
    "$ X = aU + bV$ and $Y = cU + dV$\n",
    "\n",
    "##### 1.16 Solution\n",
    "\n",
    "$Cov(X, Y) = Cov(aU + bV, cU = dV)$ \n",
    "\n",
    "$= Cov(aU, cU) + Cov (aU, dV) + Cov(bV, cU) + Cov(bV, dV)$\n",
    "\n",
    "$= acCov(U,U)+ ad(U,V) + bcCov(V,U) + bdCov(bd)$\n",
    "\n",
    "$ = acVar(U,U) + adCov(U,V) + bcCov(U,V) + bd Var(V,V)$ \n",
    "\n",
    "$ = ac + adCov(U,V) + bcCov(U,V) + bd$ `because Cov(U,V) is the covariance of independent vars,  it is zero`\n",
    "\n",
    "$ = ac + bd$\n",
    "\n"
   ]
  },
  {
   "cell_type": "markdown",
   "metadata": {},
   "source": [
    "#### 1.19 \n",
    "\n",
    "Can you construct a pair of random variables such that $Var(X) = Var(Y) = 1$, and $Cov(X, Y) = 2$?\n",
    "\n",
    "##### 1.19 Solution \n",
    "\n",
    "`Answer is no`\n",
    "\n",
    "Because \n",
    "\n",
    "$-1< \\le \\rho(X,Y) \\le 1$ \n",
    "\n",
    "and $\\rho(X,Y) = \\frac{Cov(X,Y)}{\\sqrt{Var(X)Var(Y)}}$\n",
    " \n",
    "thus $-1 \\le \\frac{Cov(X,Y)}{\\sqrt{Var(X)Var(Y)}} \\le 1$ \n",
    "\n",
    "$= -1 \\le \\frac{2}{\\sqrt{1 \\cdot 1}} \\le 1$  \n",
    "\n",
    "$ -1 \\le 2 \\le 1$ whichi is an impossible inequality"
   ]
  },
  {
   "cell_type": "markdown",
   "metadata": {},
   "source": [
    "#### 1.21\n",
    "\n",
    "The distribution function $F(x)$ of the random variable X is defined by \n",
    "\n",
    "$F(x) = P(X \\le x)$\n",
    "\n",
    "If $X$ takes on one of the values $1,2, \\ldots,$ and $F$ is a known function, how would you obtain $P(X = i)?$\n",
    "\n",
    "##### 1.21 Solution \n",
    "\n",
    "\n",
    "$P(X = i) = F(1) - F(1 - i)$\n",
    "\n",
    "\n"
   ]
  },
  {
   "cell_type": "code",
   "execution_count": null,
   "metadata": {},
   "outputs": [],
   "source": []
  }
 ],
 "metadata": {
  "kernelspec": {
   "display_name": "Python 3",
   "language": "python",
   "name": "python3"
  },
  "language_info": {
   "codemirror_mode": {
    "name": "ipython",
    "version": 3
   },
   "file_extension": ".py",
   "mimetype": "text/x-python",
   "name": "python",
   "nbconvert_exporter": "python",
   "pygments_lexer": "ipython3",
   "version": "3.7.3"
  }
 },
 "nbformat": 4,
 "nbformat_minor": 4
}
